\def\CTeXPreproc{Created by ctex v0.2.11, don't edit!}\section*{APPENDIX B}
Model equations
 \bes
\frac{dx_{1}}{dt} &=& -k_{2} x_{1} x_{2}+k_{1} x_{3}-k_{4} x_{1}
x_{4}+k_{3} x_{5},\quad
\frac{dx_{2}}{dt} = -k_{2} x_{1} x_{2}+k_{1} x_{3}-k_{5} x_{5} x_{2}-k_{6} x_{6} x_{2}-k_{7} x_{7} x_{2}\nnu\\
\frac{dx_{3}}{dt} &=& k_{2} x_{1} x_{2}-k_{1} x_{3}, \quad\quad\quad\quad \quad\quad\quad \frac{dx_{4}}{dt} = -k_{4} x_{1} x_{4}+k_{3} x_{5}+k_{5} x_{5} x_{2}+k_{6} x_{6} x_{2}+k_{7} x_{7} x_{2}\nnu\\
\frac{dx_{5}}{dt} &=& k_{4} x_{1} x_{4}-k_{3} x_{5}-k_{9} x_{5}
x_{8}+k_{8} x_{9}-k_{12} x_{5} x_{6}+k_{11} x_{10}-k_{14} x_{5}
x_{11}+k_{13} x_{12}-k_{37} x_{5} x_{27}\nnu\\
&\ &-k_{42} x_{5} x_{29}+k_{15} x_{12}\nnu\\
\frac{dx_{6}}{dt} &=& -k_{12} x_{5} x_{6}+k_{11} x_{10}-k_{28} x_{6} x_{22}+k_{27} x_{23}-k_{34} x_{6} x_{26}+k_{33} x_{27}-k_{38} x_{6} x_{29}+k_{22} x_{18}\nnu\\
\frac{dx_{7}}{dt} &=& k_{16} x_{6} x_{14}+k_{32} x_{25}
x_{23}-k_{41} x_{7} x_{29},\quad
\frac{dx_{8}}{dt} = -k_{9} x_{5} x_{8}+k_{8} x_{9}-k_{21} x_{17} x_{8}+k_{20} x_{18}+k_{25} x_{18}\nnu\\
\frac{dx_{9}}{dt} &=& k_{9} x_{5} x_{8}-k_{8} x_{9}-k_{10}
x_{9},\quad\quad\quad\frac{dx_{10}}{dt} = k_{12} x_{5} x_{6}-k_{11} x_{10}-k_{36} x_{10} x_{26}+k_{35} x_{28}+k_{10} x_{9}\nnu\\
\frac{dx_{11}}{dt} &=& -k_{14} x_{5} x_{11}+k_{13}
x_{12},\quad\quad\quad\quad\frac{dx_{12}}{dt} = k_{14} x_{5}
x_{11}-k_{13} x_{12}-k_{15}
x_{12}\nnu\\
\frac{dx_{13}}{dt} &=& -k_{19} x_{16} x_{13}+k_{18} x_{17}+k_{25}
x_{18}+k_{25} x_{17}-k_{40} x_{13} x_{29}+k_{15} x_{12}\nnu\\
\frac{dx_{14}}{dt} &=& -k_{16} x_{6} x_{14}-k_{30} x_{23}
x_{14}+k_{29} x_{24}\nnu\\ \frac{dx_{15}}{dt} &=& -k_{17} x_{7}
x_{15},\quad\quad\quad\quad\quad\frac{dx_{16}}{dt} = k_{17} x_{7}
x_{15}-k_{19}
x_{16} x_{13}+k_{18} x_{17}-k_{24} x_{16}+k_{23} x_{19} x_{20}\nnu\\
\frac{dx_{17}}{dt} &=& k_{19} x_{16} x_{13}-k_{18} x_{17}-k_{21}
x_{17} x_{8}+k_{20} x_{18}-k_{25} x_{17}+k_{22} x_{18}\nnu\\
\frac{dx_{18}}{dt} &=& k_{21} x_{17} x_{8}-k_{20} x_{18}-k_{25} x_{18}-k_{22} x_{18}\nnu\\
\frac{dx_{19}}{dt} &=& \frac{dx_{20}}{dt} ~=~ k_{24} x_{16}-k_{23} x_{19} x_{20}+k_{25} x_{18}+k_{25} x_{17}\nnu\\
\frac{dx_{21}}{dt} &=& -k_{26} x_{7} x_{21}\quad\quad\quad\quad\quad\quad\frac{dx_{22}}{dt} = k_{26} x_{7} x_{21}-k_{28} x_{6} x_{22}+k_{27} x_{23}\nnu\\
\frac{dx_{23}}{dt} &=& k_{28} x_{6} x_{22}-k_{27} x_{23}-k_{30}
x_{23} x_{14}+k_{29} x_{24}+k_{31} x_{24}\nnu\\
\frac{dx_{24}}{dt} &=& k_{30} x_{23} x_{14}-k_{29} x_{24}-k_{31}
x_{24},\quad\quad\frac{dx_{25}}{dt} = -k_{32} x_{25} x_{23}-k_{39}
x_{25} x_{29}+k_{31} x_{24}\nnu\\\frac{dx_{26}}{dt} &=& -k_{34}
x_{6}
x_{26}+k_{33} x_{27}-k_{36} x_{10} x_{26}+k_{35} x_{28}\nnu \\
\frac{dx_{27}}{dt} &=& k_{34}
x_{6} x_{26}-k_{33} x_{27}-k_{37} x_{5} x_{27},\quad\quad\frac{dx_{28}}{dt} = k_{36} x_{10} x_{26}-k_{35} x_{28}+k_{37} x_{5} x_{27}\nnu\\
\frac{dx_{29}}{dt} &=& -k_{38} x_{6} x_{29}-k_{39} x_{25} x_{29}-k_{40} x_{13} x_{29}-k_{41} x_{7} x_{29}-k_{42} x_{5} x_{29}\quad\quad\quad\frac{dx_{30}}{dt} = k_{38} x_{6} x_{29}\nnu\\
\frac{dx_{31}}{dt} &=& k_{39} x_{25}
x_{29},\quad\quad\frac{dx_{32}}{dt} = k_{40} x_{13}
x_{29},\quad\quad\quad\frac{dx_{33}}{dt} = k_{41} x_{7}
x_{29},\quad\quad\quad\frac{dx_{34}}{dt} = k_{42} x_{5}
x_{29}\label{1},\ees where $k_i,i=1,2,...,42$ are constants, and
$x_i,i=1,2,...,34$ are variables representing the species (see
Table~\ref{tabb}). The steady state system can be obtained by taking
$t\rightarrow \infty$, i.e., $\frac{dx_i}{dt}=0,\forall i$.
